\section{Fourier Transform}
Represent any function in terms of a new basis with basis vectors \(e^{-2\pi i(ux + vy)} = \cos(2\pi(ux + uv)) + i \sin(2\pi(ux + uv))\).

\begin{definition}[1D-FT]
  \(g(x) \overset{FT}{\to} \F(g)(u) = \int_{\R} g(x) e^{-i2\pi ux} \, dx\)
\end{definition}

\begin{definition}[2D-FT]
  \(g(x, y) \overset{FT}{\to} \F(g)(u, v) = \iint_{\R^2} g(x, y) e^{-i2\pi (ux + vy)} \,dx \,dy\)
\end{definition}

\begin{definition}[Inverse FT]
  \(g(x, y) = \iint_{\R^2} \F(g)(u, v) e^{i2\pi(ux + uy)} \,du \,dv\)
\end{definition}

\begin{definition}[Dirac Delta]
  \(\delta(x) = \begin{cases}
    0 & x \neq 0 \\
    \text{undefined} & x = 0
  \end{cases} \ \text{s.t.} \ \int_{\R} \delta(x) \,dx = 1\)
\end{definition}

\begin{theorem}
  \begin{itemize*}
    \item \(\delta(K - k) = \int_{\R} e^{2 \pi i (K - k)x \,dx}\)
    \item \(\delta(x) = \delta(-x)\) \\
    \item \(\delta({\color{red} \alpha} + {\color{orange} \beta}) = \int_{\R}e^{2 \pi i ({\color{red}\alpha}) x} e^{-2\pi i({\color{orange}\beta})x}\, dx\)
  \end{itemize*}
\end{theorem}

\begin{definition}[Sin and Cos identities]
  \makecell{\(e^{ix} = \cos(x) = i \sin(x)\)}
  \makecell{\(\sin(z) = \frac{e^{iz} - e^{-iz}}{2i}\)}
  \makecell{\(\cos(z) = \frac{e^{iz} + e^{-iz}}{2}\)}
\end{definition}

\subsection{Properties of the Fourier Transform}

\begin{definition}[Lin.]
  \(\F(\alpha f(x) + \beta g(x))(u) = \alpha \F(f(x))(u) + \beta \F(g(x))(u)\)
\end{definition}

\begin{definition}[Time-Shift]
  \(\F(f(t - t_0))(u) = e^{-2 \pi iwt_0 } F(u)\)
\end{definition}

\begin{definition}[Frequency-Shift]
  \(\F(e^{2 \pi iu_0t}f(t))(u) = F(u - u_0)\)
\end{definition}

\begin{algorithm}[Convolution Theorem]
  Convolution in img space is multiplication in frequency space: \(F \cdot G = \F(f \ast g)\), \(F \ast G = \F(f \cdot g)\)
\end{algorithm}

\begin{definition}[Unit Impulse]
  \(\F(\delta(x - x_0))(u) = e^{-2\pi i u x_0}\), \(\delta \ast f = f\)
\end{definition}

\begin{definition}[Sifting Property]
  \(\int_{\R} f(x)\delta(x - a) \,dx = f(a)\)
\end{definition}

\begin{definition}[FT on separable signal]
  If \(f\) is separable (\(x, y\) independent), then \(\F(f)(u, x) = \F(f_x)(x) \cdot \F(f_y)(y)\).
\end{definition}

\begin{definition}[Function Scale]
  Scale function down \(\iff\) scale transform up
\end{definition}

\begin{definition}[Gaussian]
  FT of Gaussian is Gaussian
\end{definition}

\begin{definition}[Smoothing]
  Before sampling remove high frequencies by multiply filter with signal in Fourier domain.
  Box filter is bad, as kernel has infinite support.
\end{definition}

\subsection{Fourier Transform on Images}

Consider the basis function \(B_{u,v}(x, y) = e^{-2\pi i(ux + vy)}\), then

\begin{itemize*}
  \item Magnitude of \((u, v) \sim\) frequency
  \item Direction of \(\sim\) orientation
\end{itemize*}

\begin{definition}[FT on Images]
 \(F = Uf\), where \(f\) is image and \(U\) the Fourier transform base.
 \(\F(u,v) = \sum_{x = 0}^{N - 1}\sum_{y = 0}^{M - 1} f(x, y) e^{-2\pi i (\frac{x}{N}u + \frac{y}{M}v)}\).
\end{definition}

\begin{theorem}
  All images have about the same magnitude transform.
\end{theorem}

\begin{definition}[Magnitude of \(z \in \C\)]
  \(|z| = \sqrt{z \overline{z}} = \sqrt{a^2 + b^2}\)
\end{definition}

\begin{definition}[Phase of \(z \in \C\)]
  \(\phi{z} = \arctan(\frac{b}{a})\) with case distinctions.
\end{definition}

\subsection{Sampling}
Go from continuous function to discrete vector.

\begin{definition}[Mathematical Description]
  \(\int_{\R}f(x)\delta(x - a) \,dx = f(a)\). Thus sampling is equivalent to multiplying it by the Dirac delta.
\end{definition}

\begin{definition}[Image Sampling]
  Discrete 2D-sampling
  \[\begin{aligned} \operatorname{S}_{2 \mathrm{D}}(f(x, y)) & =\sum_{i=-\infty}^{\infty} \sum_{j=-\infty}^{\infty} f(x, y) \delta(x-i, y-j) \\ & =f(x, y) \sum_{i=-\infty}^{\infty} \sum_{j=-\infty}^{\infty} \delta(x-i, y-j)\end{aligned}\]
\end{definition}

\begin{definition}[Fourier transform of a sampled signal]
  \begin{align*}
    \F\left(\operatorname{S}_{2 \mathrm{D}}(f(x, y))\right) & = \F(f(x, y)) \ast \F\left(\sum_{i} \sum_{j} \delta(x-i, y-j)\right) \\
    & = \sum_i \sum_j \F(u - i, v - j)
  \end{align*}
\end{definition}

\begin{algorithm}[Nyquist Sampling Theorem]
  Sampling frequency must be at least twice the highest frequency: \(\omega_S \geq 2 \cdot \omega\). If not the case, the signal needs to be bandlimited before sampling.
\end{algorithm}

\textbf{Proof}:
Sampling with frequency \(\omega\) involves elementwise multiplication of the signal \(h\) by a grid \(g\) with equal spaces of \(1/\omega\).
By the convolution theorem, the Fourier Transform of \(h \cdot g\) is the convolution \(H * G\), where \(H = \mathcal{F}(h)\) and \(G = \mathcal{F}(g)\).
If the signal \(h\) has a maximal frequency \(\omega_{\text{max}}\), its Fourier Transform \(H\) ranges between \(-\omega_{\text{max}}\) and \(\omega_{\text{max}}\).
The Fourier Transform of a grid \(g\) with spaces \(1/\omega\) is another grid \(G\) with spaces \(\omega\).
Convolution of the spectrum \(H\) with \(G\) copies it in the frequency domain, shifting by \(\omega\).
If \(\omega\) is smaller than \(2\omega_{\text{max}}\), overlapping spectra occur, preventing the reconstruction of the original signal \(h\).

\begin{theorem}
  To remove aliasing from cameras, change focus!
\end{theorem}

\subsection{Image Restoration Problem}
\begin{center}
  \(f(x) \to h(x) \to g(x) \to \tilde{h}(x) \to f(x)\)
\end{center}
The "inverse" kernel \(\tilde{h}(x)\) should compensate \(h(x)\). May be determined by: \(\F(\tilde{h})(u, v) \cdot \F(h)(u, v) = 1\). Convolution with kernel \(h\) may cancel out some frequencies \& noise amplification. Avoided with regularization: \(\tilde{\F}(\tilde{h})(u, v) = \frac{\F(h)}{|\F(h)|^2 + \epsilon}\).

\subsection{Transformation Examples}
\includegraphics*[width=\linewidth]{assets/fourier-functions.png}
