\section{List of distributions}
\subsection{Discrete}
\begin{center}
	\begin{tabularx}{\textwidth}{llXXXX}
		\toprule 
		Distribution & Parameters & \(\E(X)\) & \(\Var(X)\) & \(p_X(t)\) & \(F_X(t)\) \\
		\midrule
		Uniform & \makecell[l]{\(n\): \#Events \\ \(x_i\): Events} & \(\frac{1}{n} \sum_{i=1}^{n} x_i\) & \(\frac{1}{n} \sum_{i=1}^{n} x_i^2 - \frac{1}{n^2} \left(\sum_{i=1}^{n} x_i \right)^2\) & \(\frac{1}{n}\) & \(\frac{|\{k:x_k \leq t\}|}{n}\) \\
		Bernoulli & \(p:\) Probability & \(p\) & \(p \cdot (1-p)\) & \(p^t(1-p)^{1-t}\) & \(1-p\) where \(0 \leq t < 1\) \\
		Binomial & \makecell[l] {\(n\): \#Tries \\ \(p:\) Probability} & \(np\) & \(np(1-p)\) & \(\binom{n}{t}p^t(1-p)^{n-t}\) & \(\sum_{k=0}^{t} \binom{n}{k} p^k(1-p)^{n-k}\) \\
		Geometric & \makecell[l] {\(p\): Probability \\ \(t:\) \#Tries} & \(\frac{1}{p}\) & \(\frac{1-p}{p^2}\) & \(p(1-p)^{t-1}\) & \(1-(1-p)^t\) \\
		Poisson          & \makecell[l]{ \(\lambda\): Lambda} & \(\lambda\) & \(\lambda\) & \(\frac{\lambda^t}{t!}e^{-\lambda}\) & \(e^{-\lambda} \sum_{k=0}^{t} \frac{\lambda^{k}}{k!}\) \\
		\bottomrule
	\end{tabularx}
\end{center}

\subsection{Continuous}
\begin{center}
	\begin{tabularx}{\textwidth}{llXXXX}
		\toprule
		Distribution & Parameters & \(\E(X)\) & \(\Var(X)\) & \(f_X(t)\)                                                                                                                                  & \(F_X(t)\) \\
		\midrule
		Uniform & \([a,b]\): Intervall & \(\frac{a+b}{2}\) & \(\frac{1}{12}(b-a)^2\) & \(\begin{cases} \frac{1}{b-a} &a \le t \le b \\ 0 & \text{otherwise}\end{cases}\) & \(\begin{cases} 0 & t\le a \\ \frac{t-a}{b-a} & a < t < b \\ 1 & t \ge b \end{cases}\) \\
		Exponential & \(\lambda: \frac{1}{\E(X)}\) & \(\frac{1}{\lambda}\) & \(\frac{1}{\lambda^2}\) & \(\begin{cases} \lambda e^{-\lambda t} & t \geq 0 \\ 0 & t < 0 \end{cases}\) & \(\begin{cases} 1-e^{-\lambda t} & t>0 \\ 0 & t \leq 0\end{cases}\) \\
		Normal & \makecell[l]{\(\sigma^2\): Variance \\ \(\mu: \E(X)\)} & \(\mu\) & \(\sigma ^2\) & \(\frac{1}{\sqrt{2\pi \sigma^2} }e^{-{\frac{(t-\mu)^2}{2\sigma^2} }}\) & \(\frac{1}{\sigma {\sqrt{2\pi}}} \int_{-\infty}^t e^{-\frac{1}{2}\left( \frac{y-\mu}{\sigma} \right) ^2} \mathrm{d} y\) \\
		\bottomrule
	\end{tabularx}
\end{center}
