\section{Kernel Trick}
As \(w \in \Im(\Phi^\top) \Rightarrow w = \Phi^\top \alpha; \ K_{i, j} = k(x_i, x_j)\).
Conditions for a valid kernel function \(k\): \\
\begin{itemize*}
  \item \(k(x, z) = k(z, x)\)
  \item \(K\) psd s.t. \(\forall x. \ x^\top K x \geq 0 \) \\
\end{itemize*}
Want to find map \(\phi\) s.t. \(k(x, y) = \langle\phi(x), \phi(y)\rangle\).

\begin{definition}[Inner Product kernel]
  \(k(x, z) = h(\langle x, z \rangle)\)
\end{definition}

\begin{definition}[Polynomial kernel]
  \(k(x, z) = (1 + \langle x, z \rangle)^m\)
\end{definition}

\begin{definition}[RFB kernel]
  \(k(x, z)  = \exp\left(\frac{||x - z||_2^\alpha}{\tau}\right)\) which is \textbf{Gaussian} if \(\alpha = 2\), \textbf{Laplacian} if \(\alpha = 1\).
\end{definition}

\begin{definition}[Kernel Composition]
  \begin{itemize*}
    \item \(k_1 \dotplus k_2\)
    \item \(c\cdot k \ (c >0)\)
    \item \(k((x \ y), (x' \ y')) = k_1(x \ x') \dotplus k_2(y \ y') \)
  \end{itemize*}
\end{definition}

\begin{definition}[Kernelized Ridge]
  \(\frac{1}{n}||y - K\alpha||^2 + \lambda \alpha^\top K \alpha\)
  The final model is \(\hat{f}(x) = \hat{\alpha}^\top [k(x_i, x)]_i\).
\end{definition}